\begin{equation}
	a_l \left( \frac{a}{2} \delta_{lk} + \frac{2}{b} \sum\limits_{m = 1}^{+\infty} \frac{1}{\gamma_{m}} J^a_{l,m} I^a_{k,m} \right) + \sum\limits_{n = 1}^{+\infty} b^1_n \left( \frac{a}{2} \delta_{kn} - \gamma_{an} \frac{2}{b} \sum\limits_{m = 1}^{+\infty} \frac{1}{\gamma_{m}} J^a_{n,m} I^a_{k,m} \right) = 2 \sum\limits_{n = 1}^{+\infty}a^5_n I^a_{n, k}
\end{equation}

\begin{equation}
	\sum\limits_{n = 1}^{+\infty} b^3_n \left( \frac{b-a}{2} \delta_{kn} - \gamma_{bn} \frac{2}{b} \sum\limits_{m = 1}^{+\infty} \frac{1}{\gamma_{m}} J^b_{n,m} I^b_{k,m} \right) = 2 \sum\limits_{n = 1}^{+\infty}a^5_n I^b_{n, k}
\end{equation}

\begin{equation}
	\sum\limits_{n = 1}^{+\infty} a^2_n e^{i\gamma_{an}c} \left( \frac{a}{2} \delta_{kn} + \gamma_{an} \frac{2}{b} \sum\limits_{m = 1}^{+\infty} \frac{1}{\gamma_{m}} J^a_{n,m} I^a_{k,m} \right) = 2 \sum\limits_{n = 1}^{+\infty}a^5_n e^{i\gamma_{n}c} I^a_{n, k}
\end{equation}

\begin{equation}
	\sum\limits_{n = 1}^{+\infty} a^4_n e^{i\gamma_{bn}c} \left( \frac{b-a}{2} \delta_{kn} + \gamma_{bn} \frac{2}{b} \sum\limits_{m = 1}^{+\infty} \frac{1}{\gamma_{m}} J^b_{n,m} I^b_{k,m} \right) = 2 \sum\limits_{n = 1}^{+\infty}a^5_n e^{i\gamma_{n}c} I^b_{n, k}
\end{equation}